Restore interop for decrypt (remove admit_smt_queries in makefile)

vale/code/arch/x64/interop/Vale.Wrapper.X64.GCMdecryptOpt.fsti
@@ -109,17 +109,19 @@ let decrypt_opt_stdcall_st (a: algorithm { a = AES_128 \/ a = AES_256 }) =
         (seq_nat8_to_seq_uint8 (le_seq_quad32_to_bytes (key_to_round_keys_LE a (Ghost.reveal key))))) /\
 
       hkeys_reqs_pub (le_bytes_to_seq_quad32 (seq_uint8_to_seq_nat8 (B.as_seq h0 hkeys_b)))
-        (reverse_bytes_quad32 (aes_encrypt_LE a (Ghost.reveal key) (Mkfour 0 0 0 0)))
+        (reverse_bytes_quad32 (aes_encrypt_LE a (Ghost.reveal key) (Mkfour 0 0 0 0))) /\
+
+      (be_bytes_to_quad32 (seq_uint8_to_seq_nat8 (B.as_seq h0 iv_b)) ==
+        compute_iv_BE (aes_encrypt_LE a (Ghost.reveal key) (Mkfour 0 0 0 0)) (Ghost.reveal iv))
     )
     (ensures fun h0 c h1 ->
       B.modifies (B.loc_union (B.loc_buffer iv_b)
                  (B.loc_buffer out_b)) h0 h1 /\
 
-      (let iv = seq_uint8_to_seq_nat8 (B.as_seq h0 iv_b) in
-       let cipher = seq_uint8_to_seq_nat8 (B.as_seq h0 cipher_b) in
+      (let cipher = seq_uint8_to_seq_nat8 (B.as_seq h0 cipher_b) in
        let auth = seq_uint8_to_seq_nat8 (B.as_seq h0 auth_b) in
        let expected_tag = seq_uint8_to_seq_nat8 (B.as_seq h0 tag_b) in
-       let plain, result = gcm_decrypt_LE a (seq_nat32_to_seq_nat8_LE (Ghost.reveal key)) iv cipher auth expected_tag in
+       let plain, result = gcm_decrypt_LE a (seq_nat32_to_seq_nat8_LE (Ghost.reveal key)) (Ghost.reveal iv) cipher auth expected_tag in
        Seq.equal (seq_uint8_to_seq_nat8 (B.as_seq h1 out_b)) plain /\
        (UInt64.v c = 0) == result)
   )
